Use FuseIfte

Minimp/Equiv.v
@@ -27,6 +27,70 @@ Module Type EQUIV
       stmt_eval prog menv env s1 (menv', env')
       <->
       stmt_eval prog menv env s2 (menv', env').
+  
+  Axiom stmt_eval_eq_refl:
+    reflexive stmt stmt_eval_eq.
+  
+  Axiom stmt_eval_eq_sym:
+    symmetric stmt stmt_eval_eq.
+  
+  Axiom stmt_eval_eq_trans:
+    transitive stmt stmt_eval_eq.
+  
+  Add Relation stmt (stmt_eval_eq)
+      reflexivity proved by stmt_eval_eq_refl
+      symmetry proved by stmt_eval_eq_sym
+      transitivity proved by stmt_eval_eq_trans
+        as stmt_eval_equiv.
+
+  Instance stmt_eval_eq_Proper:
+    Proper (eq ==> eq ==> eq ==> stmt_eval_eq ==> eq ==> iff) stmt_eval.
+  Proof.
+    intros prog' prog HR1 menv' menv HR2 env' env HR3 s1 s2 Heq r' r HR4;
+    subst; destruct r as [menv' env'].
+    now apply Heq.
+  Qed.
+
+  Instance stmt_eval_eq_Comp_Proper:
+    Proper (stmt_eval_eq ==> stmt_eval_eq ==> stmt_eval_eq) Comp.
+  Proof.
+    intros s s' Hseq t t' Hteq prog menv env menv' env'.
+    split; inversion_clear 1;
+    [rewrite Hseq, Hteq in *; econstructor; eassumption
+    |rewrite <-Hseq, <-Hteq in *; econstructor; eassumption].
+  Qed.
+
+  Axiom Comp_assoc:
+    forall s1 s2 s3,
+      stmt_eval_eq (Comp s1 (Comp s2 s3)) (Comp (Comp s1 s2) s3).
+ 
+  Axiom stmt_eval_eq_Comp_Skip1:
+    forall s, stmt_eval_eq (Comp Skip s) s.
+  
+  Axiom stmt_eval_eq_Comp_Skip2:
+    forall s, stmt_eval_eq (Comp s Skip) s.
+  
+  Instance stmt_eval_eq_Ifte_Proper:
+    Proper (eq ==> stmt_eval_eq ==> stmt_eval_eq ==> stmt_eval_eq) Ifte.
+  Proof.
+    intros e e' Heeq s s' Hseq t t' Hteq prog menv env menv' env'.
+    rewrite <-Heeq.
+    split; inversion_clear 1; apply Iifte with b; auto; destruct b;
+    [now rewrite <-Hseq | now rewrite <-Hteq | now rewrite Hseq | now rewrite Hteq].
+  Qed.
+
+End EQUIV.
+
+Module EquivFun'
+       (Op : OPERATORS)
+       (Import Syn : SYNTAX Op)
+       (Import Sem : SEMANTICS Op Syn).
+  
+  Definition stmt_eval_eq s1 s2: Prop :=
+    forall prog menv env menv' env',
+      stmt_eval prog menv env s1 (menv', env')
+      <->
+      stmt_eval prog menv env s2 (menv', env').
 
   Lemma stmt_eval_eq_refl:
     reflexive stmt stmt_eval_eq.
@@ -116,4 +180,5 @@ Module Type EQUIV
     [now rewrite <-Hseq | now rewrite <-Hteq | now rewrite Hseq | now rewrite Hteq].
   Qed.
 
-End EQUIV.
+End EquivFun'.
+Module EquivFun <: EQUIV := EquivFun'.
