Minimp.v
@@ -3,8 +3,9 @@ Require Export Minimp.Semantics.
 Require Export Minimp.Equiv.
 
 Require Import Rustre.Common.
+
 Module Type MINIMP (Op: OPERATORS).
   Declare Module Export Syn: SYNTAX Op.
   Declare Module Export Sem: SEMANTICS Op Syn.
   Declare Module Export Equ: EQUIV Op Syn Sem.
- End MINIMP.
+End MINIMP.
